{
 "cells": [
  {
   "cell_type": "markdown",
   "id": "f4c96e54-5e29-498d-93bc-2f1b6c5404aa",
   "metadata": {},
   "source": [
    "# Solving Non-Singular Systems of Linear Equations"
   ]
  },
  {
   "cell_type": "markdown",
   "id": "ae1d990a-9808-42b6-b8a9-6daee3f7e20b",
   "metadata": {},
   "source": [
    "We are now ready to learn a formal algorithm for finding the solution to a system of linear equations. This method will allow us to solve any non-singular system and will also help us identify if a system is singular.\n",
    "\n",
    "Let's start by revisiting the apple and banana problem:\n",
    "\n",
    "1.  $a + b = 10$\n",
    "2.  $a + 2b = 12$\n",
    "\n",
    "Our logical deduction led us to the **solved system**:\n",
    "\n",
    "1.  $a = 8$\n",
    "2.  $b = 2$\n",
    "\n",
    "The goal of this lesson is to learn a systematic process to get from any non-singular system to its solved version. This process involves manipulating the equations in specific, allowed ways.\n",
    "\n",
    "---\n",
    "\n",
    "## Allowed Equation Manipulations\n",
    "\n",
    "There are two primary ways we can manipulate linear equations to create new, equally true equations.\n",
    "\n",
    "1.  **Multiplying by a Constant:** If an equation is true, multiplying both sides by the same non-zero constant results in an equation that is also true and carries the same information.\n",
    "    * **Example:** If $a + b = 10$, then it is also true that $7(a+b) = 7(10)$, which gives us $7a + 7b = 70$.  \n",
    "` `\n",
    "2.  **Adding Two Equations:** If two separate equations are true, their sum is also a true equation.\n",
    "    * **Example:** If $a + b = 10$ and $2a + 3b = 26$ are both true, then adding them together gives us the new true equation $(a+2a) + (b+3b) = 10+26$, which simplifies to $3a + 4b = 36$.\n",
    "\n",
    "---\n",
    "\n",
    "## Solving a System: A Step-by-Step Example\n",
    "\n",
    "Let's use these manipulations to solve a slightly harder system of equations. Our goal is to eliminate one variable from one of the equations.\n",
    "\n",
    "**System:**\n",
    "1.  $5a + b = 17$\n",
    "2.  $4a - 3b = 6$\n",
    "\n",
    "\n",
    "### Step 1: Normalize the 'a' Coefficient\n",
    "\n",
    "To make subtraction easier, let's make the coefficient of `a` equal to 1 in both equations. We do this by dividing each equation by its `a` coefficient.\n",
    "\n",
    "* **Equation 1:** Divide by 5 ➔ $a + 0.2b = 3.4$\n",
    "* **Equation 2:** Divide by 4 ➔ $a - 0.75b = 1.5$\n",
    "\n",
    "Our new, equivalent system is:\n",
    "1.  $a + 0.2b = 3.4$\n",
    "2.  $a - 0.75b = 1.5$\n",
    "\n",
    "### Step 2: Eliminate 'a' from the Second Equation\n",
    "\n",
    "Now we can subtract the first new equation from the second new equation to eliminate `a`.\n",
    "\n",
    "$ (a - a) + (-0.75b - 0.2b) = (1.5 - 3.4) $  \n",
    "$ 0a - 0.95b = -1.9 $  \n",
    "$ -0.95b = -1.9 $  \n",
    "\n",
    "\n",
    "### Step 3: Solve for 'b'\n",
    "\n",
    "Now that `a` is gone, we have a simple equation with only one unknown.\n",
    "\n",
    "$ -0.95b = -1.9 $  \n",
    "$ b = \\frac{-1.9}{-0.95} $  \n",
    "$ b = 2 $  \n",
    "\n",
    "We have found the first part of our solution!\n",
    "\n",
    "\n",
    "### Step 4: Substitute to Find 'a'\n",
    "\n",
    "Now that we know `b = 2`, we can substitute this value back into one of our simplified original equations (let's use the first one).\n",
    "\n",
    "$ a + 0.2b = 3.4 $  \n",
    "$ a + 0.2(2) = 3.4 $  \n",
    "$ a + 0.4 = 3.4 $  \n",
    "$ a = 3.4 - 0.4 $  \n",
    "$ a = 3 $  \n",
    "\n",
    "\n",
    "### The Solved System\n",
    "\n",
    "We have successfully transformed our original system into the solved system:\n",
    "1.  $a = 3$\n",
    "2.  $b = 2$\n",
    "\n",
    "---\n",
    "\n",
    "## A Special Case: Zero Coefficients\n",
    "\n",
    "What if the variable you want to eliminate is already missing from an equation?\n",
    "\n",
    "**New System:**\n",
    "1.  $5a + b = 17$\n",
    "2.  $3b = 6$\n",
    "\n",
    "Here, the coefficient of `a` in the second equation is 0. This is good news! The variable `a` is already eliminated for us. We can immediately solve the second equation:\n",
    "\n",
    "$ 3b = 6 \\implies b = 2 $\n",
    "\n",
    "We can then proceed with Step 4 as usual, substituting `b=2` into the first equation to find that `a=3`."
   ]
  }
 ],
 "metadata": {
  "kernelspec": {
   "display_name": "Python 3 (ipykernel)",
   "language": "python",
   "name": "python3"
  },
  "language_info": {
   "codemirror_mode": {
    "name": "ipython",
    "version": 3
   },
   "file_extension": ".py",
   "mimetype": "text/x-python",
   "name": "python",
   "nbconvert_exporter": "python",
   "pygments_lexer": "ipython3",
   "version": "3.13.5"
  }
 },
 "nbformat": 4,
 "nbformat_minor": 5
}
